Add definition-level documentation

examples/kv_parsing/Serializing.fst
@@ -18,6 +18,19 @@ module U16 = FStar.UInt16
 module U32 = FStar.UInt32
 module Cast = FStar.Int.Cast
 
+(* Note the lack of definitions around encoding, the pure specification for serialization.
+
+   An encoded value is simply of type [bytes] ([seq byte]). Encoders are
+   functions from whatever they encode to [Tot bytes]. There should be no need for
+   failures during encoding, due to restrictions in the types or
+   refinements/preconditions on the encoders themselves.
+
+   Note that no connection is made here to parsing. Instead, this can be done
+   outside this library by relating the pure parsers to the pure encoders.
+
+*)
+
+/// Encode a list of values and concatenate the results.
 val encode_many : #t:Type -> l:list t -> enc:(t -> bytes) -> n:nat{n <= List.length l} -> bytes
 let rec encode_many #t l enc n =
   match n with
@@ -27,6 +40,10 @@ let rec encode_many #t l enc n =
 
 let offset_into (buf:bslice) = off:U32.t{U32.v off <= U32.v buf.len}
 
+/// The core specification of serialization, the stateful analogue of encoding.
+/// Note that this condition requires that only the first off bytes of the
+/// output buffer are modified if the serializer succeeds, but allows the entire
+/// output buffer to be arbitrarily modified if it fails.
 let serialized (enc:bytes) (buf:bslice) (r:option (offset_into buf)) (h0 h1:mem) :
     Pure Type0
     (requires (live h1 buf))
@@ -39,22 +56,41 @@ let serialized (enc:bytes) (buf:bslice) (r:option (offset_into buf)) (h0 h1:mem)
     | None ->
       modifies_slice buf h0 h1
 
+/// A buffer_fun captures a specification encoder that relies on a fixed set of
+/// input bslices. It is required to depend on only those bslices since it
+/// returns the same output for any two heaps where all the inputs buffers have
+/// equal abstract values. The definition is complicated to do allowing the
+/// function to assume all the input buffers are live in any heap it operates
+/// on.
 let buffer_fun (inputs:erased (TSet.set bslice)) =
     f:(h:mem{forall b. TSet.mem b (reveal inputs) ==> live h b} -> GTot bytes){
       forall (h0 h1: h:mem{forall b. TSet.mem b (reveal inputs) ==> live h b}).
       (forall b. TSet.mem b (reveal inputs) ==> as_seq h0 b == as_seq h1 b) ==>
       f h0 == f h1}
 
-let disjoint_in (h:mem) (inputs:TSet.set bslice) (buf:bslice) =
+/// Predicate that buf is disjoint from all the inputs (used to assert that the
+/// output buffer while serializing is disjoint from input buffers, since inputs
+/// are expected to be immutable while serializing).
+let disjoint_from (h:mem) (inputs:TSet.set bslice) (buf:bslice) =
   forall b. TSet.mem b inputs ==> live h b /\ B.disjoint b.p buf.p
 
+/// A general serializer, taking input from some set of buffers. The input
+/// buffers are required to be disjoint from the output and are unmodified. The
+/// definition of [serialized] enforces that the output buffer has the correct
+/// bytes.
+///
+/// As with parsers (and their stateful variants), we do not enforce a lack of
+/// lookahead (or even reading) in these serializers. A more general property
+/// not enforced here is that serializers should succeed if given a large enough
+/// input buffer (this would forbid success depending on the contents of the
+/// output buffer, for example).
 inline_for_extraction
 let serializer_any (inputs:erased (TSet.set bslice))
                    (enc: buffer_fun inputs) =
   buf:bslice ->
   Stack (option (off:offset_into buf))
      (requires (fun h0 -> live h0 buf /\
-                       disjoint_in h0 (reveal inputs) buf))
+                       disjoint_from h0 (reveal inputs) buf))
      (ensures (fun h0 r h1 ->
         live h0 buf /\
         live h1 buf /\
@@ -64,9 +100,13 @@ let serializer_any (inputs:erased (TSet.set bslice))
            as_seq h0 b == as_seq h1 b) /\
         serialized (enc h1) buf r h0 h1))
 
+/// Special case of [serializer_any] with no input buffers and thus a fixed set of
+/// bytes to be serialized. Typically the bytes to encode would be computed from
+/// the inputs by a pure encoder function.
 inline_for_extraction
 let serializer (enc:erased bytes) = serializer_any (hide TSet.empty) (fun _ -> reveal enc)
 
+/// Special case of [serializer_any] with only one input buffer.
 inline_for_extraction
 let serializer_1 (input:bslice) (enc: buffer_fun (hide (TSet.singleton input))) =
     serializer_any (hide (TSet.singleton input)) (fun h -> enc h)
@@ -87,6 +127,8 @@ let ser_inputs (#inputs1:erased (TSet.set bslice))
 
 #reset-options "--z3rlimit 30"
 
+/// Run two serializers in sequence (monoidally combines serializers). Fully
+/// general; combines the input buffer sets of the two serializers.
 [@"substitute"]
 let ser_append (#inputs1 #inputs2:erased (TSet.set bslice))
                (#b1: buffer_fun inputs1) (#b2: buffer_fun inputs2)
@@ -101,6 +143,8 @@ let ser_append (#inputs1 #inputs2:erased (TSet.set bslice))
       let buf0 = buf in
       let (buf1, buf) = bslice_split_at buf off in
       match s2 buf with
+      // TODO: this overflow should actually be impossible, since off + off' is
+      // a valid offset for the original slice, which had length < 2^32.
       | Some off' -> (if u32_add_overflows off off' then None
                      else begin
                       begin
@@ -126,6 +170,8 @@ let ser_append (#inputs1 #inputs2:erased (TSet.set bslice))
 
 #reset-options
 
+/// Simple serializer_1 that just copies the input buffer. Fails if supplied
+/// a short output buffer, and otherwise just performs a memcpy.
 [@"substitute"]
 val ser_copy : data:bslice -> serializer_1 data (fun h -> as_seq h data)
 [@"substitute"]
